implement and prove realize

Scratch.thy
@@ -2,7 +2,7 @@ theory Scratch
   imports Main "Separation_Logic_Imperative_HOL.Sep_Main" "Deriving.Derive" "HOL-Library.Code_Target_Nat"
 begin
 
-
+(* TODO Rename *)
 abbreviation member where
   "member xs x \<equiv> x \<in> set xs"
 
@@ -74,11 +74,11 @@ definition master_assn :: "('a cell ref * 'a::heap cell') list \<Rightarrow> ass
   "master_assn C = fold_assn (map (\<lambda>(p, c'). \<exists>\<^sub>A c. p \<mapsto>\<^sub>r c * cell_assn c' c) C)"
 
 
-lemma open_master_assn': "master_assn ((p,c')#xs) = (\<exists>\<^sub>A c. p \<mapsto>\<^sub>r c * cell_assn c' c) * master_assn xs"
+lemma open_master_assn_cons: "master_assn ((p,c')#xs) = (\<exists>\<^sub>A c. p \<mapsto>\<^sub>r c * cell_assn c' c) * master_assn xs"
   unfolding master_assn_def
   by auto
 
-lemma open_master_assn: 
+lemma open_master_assn': 
   assumes "member xs (p, c')"
   shows "master_assn xs = (\<exists>\<^sub>A c. p \<mapsto>\<^sub>r c * cell_assn c' c) * master_assn (remove1 (p, c') xs)"
 proof-
@@ -94,9 +94,14 @@ proof-
     by auto
 qed 
 
+lemma open_master_assn: 
+  assumes "member xs (p, c')"
+  shows "master_assn xs \<Longrightarrow>\<^sub>A (\<exists>\<^sub>A c. p \<mapsto>\<^sub>r c * cell_assn c' c) * master_assn (remove1 (p, c') xs)"
+  using assms open_master_assn' by fastforce
+
 fun la_rel' where
   "la_rel' C 0 xs a \<longleftrightarrow> member C (a, Array' xs)"
-| "la_rel' C (Suc n) xs a \<longleftrightarrow> (\<exists>i x a' xs'. member C (a, Upd' i x a') \<and> la_rel' C n xs' a' \<and> xs = xs'[i:=x])"
+| "la_rel' C (Suc n) xs a \<longleftrightarrow> (\<exists>i x a' xs'. member C (a, Upd' i x a') \<and> la_rel' C n xs' a' \<and> xs = xs'[i:=x] \<and> i < length xs')"
   
 definition la_rel where
   "la_rel C xs a \<equiv> \<exists>n. la_rel' C n xs a"
@@ -139,87 +144,211 @@ lemma [simp]:"cell_assn (Upd' i x p) c = \<up>(c = Upd i x p)"
 
 lemma close_master_assn_array: "member t (a, Array' xs) 
   \<Longrightarrow> a' \<mapsto>\<^sub>a xs * a \<mapsto>\<^sub>r cell.Array a' * master_assn (remove1 (a, Array' xs) t) \<Longrightarrow>\<^sub>A master_assn t"
-  using open_master_assn[of a "Array' xs" t]
+  using open_master_assn'[of a "Array' xs" t]
   by sep_auto
 
 lemma close_master_assn_upd: "member t (a, Upd' i x a')
      \<Longrightarrow> a \<mapsto>\<^sub>r Upd i x a' * master_assn (remove1 (a, Upd' i x a') t) \<Longrightarrow>\<^sub>A master_assn t"
-  using open_master_assn[of a "Upd' i x a'" t]
+  using open_master_assn'[of a "Upd' i x a'" t]
   by sep_auto
 
 lemma close_master_assn_upd': "member t (a, Upd' i x a')
      \<Longrightarrow> a \<mapsto>\<^sub>r Upd i x a' * master_assn (remove1 (a, Upd' i x a') t) = master_assn t"
-  using open_master_assn[of a "Upd' i x a'" t]
+  using open_master_assn'[of a "Upd' i x a'" t]
   by(auto simp: ent_iffI entails_def)
 
-(* How to inline these? *)
-lemma helper1:
-  assumes 
-    "i < length xs'"
-    "member t (a, Upd' i x a')"
-    "la_rel' t n xs' a'"
-    "xs = xs'[i := x]"
-  shows
-    "a \<mapsto>\<^sub>r Upd i x a' * master_assn (remove1 (a, Upd' i x a') t) \<Longrightarrow>\<^sub>A master_assn t * true"
-proof-  
-  from assms show ?thesis 
-    using close_master_assn_upd[of a i x a' t]
-    apply sep_auto
-    using ent_true_drop(2) by blast
-qed
 
-lemma helper2: 
-  assumes
-     "i < length xs'" 
-     "member t (a, Upd' ia x a')" 
-     "la_rel' t n xs' a'" 
-     "xs = xs'[ia := x]"
-     "i \<noteq> ia"
-   shows "
-      <a \<mapsto>\<^sub>r Upd ia x a' * master_assn (remove1 (a, Upd' ia x a') t)> lookup a' i <\<lambda>r. master_assn t * true * \<up> (r = xs' ! i)>
-       = <master_assn t> lookup a' i <\<lambda>x. master_assn t * true * \<up> (x = xs' ! i)>"
-  using close_master_assn_upd'[of a ia x a' t] assms
-  by auto
+lemma htriple_frame_fwd:
+  assumes R: "P \<Longrightarrow>\<^sub>A R"
+  assumes F: "Ps \<Longrightarrow>\<^sub>A P*F"
+  assumes I: "<R*F> c <Q>"
+  shows "<Ps> c <Q>"
+  using assms
+  by (metis cons_rule ent_refl fr_refl)
 
-lemma lookup: "<master_assn t * \<up>(la_rel' t n xs a \<and> i < length xs)> lookup a i <\<lambda>r. master_assn t * \<up>(r = xs!i)>\<^sub>t"
+method sep_drule uses r = rule ent_frame_fwd[OF r] htriple_frame_fwd[OF r], (assumption+)?, frame_inference
+
+lemma lookup_aux: "<\<up>(la_rel' t n xs a \<and> i < length xs) * master_assn t > lookup a i <\<lambda>r. master_assn t * \<up>(r = xs!i)>\<^sub>t"
 proof(induction n arbitrary: xs a)
   case 0
-  then have "\<And>a'. \<lbrakk>member t (a, Array' xs); i < length xs\<rbrakk>
-         \<Longrightarrow> a' \<mapsto>\<^sub>a xs * a \<mapsto>\<^sub>r cell.Array a' * master_assn (remove1 (a, Array' xs) t) \<Longrightarrow>\<^sub>A master_assn t"
-    using close_master_assn_array
-    by sep_auto
-
-  then show ?case
+  show ?case
     apply(sep_auto)
     apply(subst lookup.simps)
-    apply(subst open_master_assn, assumption)
+    apply(sep_drule r: open_master_assn)
     apply(sep_auto)
-    using ent_true_drop(2) by blast
+    apply (sep_drule r: close_master_assn_array)
+    by sep_auto
 next
   case (Suc n)
 
   show ?case
     apply(sep_auto)
     apply(subst lookup.simps)
-    apply(subst open_master_assn, assumption)
-    apply(sep_auto simp: helper1 helper2)
+    apply(sep_drule r: open_master_assn)
+    apply sep_auto
+    apply (sep_drule r: close_master_assn_upd)
+    apply sep_auto
+    apply (sep_drule r: close_master_assn_upd)
+    apply sep_auto
     apply (rule cons_post_rule)
     apply (rule fi_rule[OF Suc.IH])
     by sep_auto+
 qed
 
-partial_function (heap) update :: "('a::heap) la \<Rightarrow> nat \<Rightarrow> 'a::heap \<Rightarrow> 'a la Heap" where
-  "update la n v = do {
-      old_v \<leftarrow> lookup la n;
+lemma lookup: "
+  <master_assn t * \<up>(la_rel t xs a \<and> i < length xs)> 
+    lookup a i 
+  <\<lambda>r. master_assn t * \<up>(r = xs!i)>\<^sub>t
+" unfolding la_rel_def
+  apply(sep_auto)
+  apply(rule cons_post_rule)
+   apply(rule fi_rule[OF lookup_aux[of t _ xs]])
+  by(solve_entails)
+
+partial_function (heap) realize :: "('a::heap) la \<Rightarrow> 'a array Heap" where
+  "realize la = do {
+    cell \<leftarrow> !la;
+     case cell of
+        Array arr \<Rightarrow> do {
+            len \<leftarrow> Array.len arr;
+            xs  \<leftarrow> Array.freeze arr;
+            Array.make len (List.nth xs)
+        }
+      | Upd i v la \<Rightarrow> do {
+          arr \<leftarrow> realize la;
+          Array.upd i v arr
+        }
+  }"
+declare realize.simps[code]
+
+partial_function (heap) update_aux :: "('a::heap) la \<Rightarrow> nat \<Rightarrow> 'a::heap \<Rightarrow> 'a la Heap" where
+  "update_aux la i v = do {
       cell \<leftarrow> !la;
-      new_la \<leftarrow> case cell of       
-         Array array \<Rightarrow> Array.upd n v array \<bind> array_to_la
-       | Upd m w la' \<Rightarrow> 
-            do {
-                tmp \<leftarrow> update la' n v;
-                ref (Upd m w tmp)
-            };
-      la :=\<^sub>R Upd n old_v new_la;
+      arr \<leftarrow> case cell of       
+         Array arr \<Rightarrow> return arr
+       | Upd _ _ _ \<Rightarrow> realize la;
+      arr \<leftarrow> Array.upd i v arr;
+      array_to_la arr
+  }" 
+declare update_aux.simps[code]
+
+abbreviation replace :: "'a \<Rightarrow> 'a \<Rightarrow> 'a list \<Rightarrow> 'a list" where
+  "replace x y xs \<equiv> y # remove1 x xs"
+
+
+lemma array_to_la': "
+  <a \<mapsto>\<^sub>a xs * master_assn t>
+  array_to_la a      
+  <\<lambda>r. let t' = (r, Array' xs)#t 
+    in master_assn t' * \<up>(la_rel t' xs r)>"
+  unfolding array_to_la_def Let_def la_rel_def
+  apply sep_auto
+   apply (meson la_rel'.simps(1) la_rel_def list.set_intros(1))
+  by (metis close_master_assn_array list.set_intros(1) remove1.simps(2) star_aci(2))
+
+lemma realize_aux: "
+   <master_assn t * \<up>(la_rel' t n xs la)> 
+    realize la
+  <\<lambda>arr. master_assn t * \<up>(la_rel' t n xs la) * arr \<mapsto>\<^sub>a xs>
+" 
+proof(induction n arbitrary: t la xs)
+  case 0
+  then show ?case
+    apply sep_auto
+    apply(subst realize.simps)
+    apply(sep_drule r: open_master_assn)
+    apply sep_auto
+    apply(sep_drule r: close_master_assn_array)
+    by(sep_auto simp: map_nth)
+next
+  case (Suc n)
+  then show ?case
+    apply sep_auto
+    apply(subst realize.simps)
+    apply(sep_drule r: open_master_assn)
+    apply sep_auto
+    apply(sep_drule r: close_master_assn_upd)
+    apply sep_auto
+    apply(sep_drule r: open_master_assn)
+    apply sep_auto
+    apply(sep_drule r: close_master_assn_upd)
+    by sep_auto
+qed
+
+lemma realize: "
+   <master_assn t * \<up>(la_rel t xs la)> 
+    realize la
+  <\<lambda>arr. master_assn t * \<up>(la_rel t xs la) * arr \<mapsto>\<^sub>a xs>
+" 
+  unfolding la_rel_def
+  apply(sep_auto)
+  subgoal for n
+    using realize_aux[of t n xs la]
+    by sep_auto
+  done
+ 
+
+find_theorems "<_> !_ <_>"
+
+
+(* TODO: Is the c important? *)
+lemma ref_lookup': "\<lbrakk>la_rel' t n xs la\<rbrakk> \<Longrightarrow> <master_assn t> !la <\<lambda>c. master_assn t>"
+proof(induction n)
+  case 0
+  then show ?case
+    apply sep_auto
+    apply(sep_drule r: open_master_assn)
+    apply sep_auto
+    apply(sep_drule r: close_master_assn_array)
+    by sep_auto
+next
+  case (Suc n)
+  then show ?case 
+    apply sep_auto
+    apply(sep_drule r: open_master_assn)
+    apply sep_auto
+    apply(sep_drule r: close_master_assn_upd)
+    by sep_auto
+qed
+
+lemma ref_lookup: "\<lbrakk>la_rel t xs la\<rbrakk> \<Longrightarrow> <master_assn t> !la <\<lambda>c. master_assn t >"
+  unfolding la_rel_def
+  using ref_lookup'
+  by sep_auto
+
+
+lemma update_aux: "
+  <master_assn t * \<up>(la_rel t xs la \<and> i < length xs)> 
+    update_aux la i v
+  <\<lambda>la. master_assn t * \<up>(la_rel t (xs[i := v]) la)>
+"
+  apply(subst update_aux.simps)
+  apply sep_auto
+   apply(rule fi_rule[OF ref_lookup])
+    apply sep_auto+
+  apply(sep_auto split: cell.splits)
+   apply (rule cons_post_rule)
+  
+  thm realize[of t ]
+    apply (rule fi_rule[OF realize])
+    apply sep_auto+
+ 
+  thm upd_rule[of i xs _ v]
+   apply (rule fi_rule[OF upd_rule[of i xs _ v], of ])
+    apply sep_auto
+  unfolding la_rel_def
+   apply sep_auto
+  subgoal
+    sorry
+  by sep_auto
+  
+
+
+partial_function (heap) update :: "('a::heap) la \<Rightarrow> nat \<Rightarrow> 'a::heap \<Rightarrow> 'a la Heap" where
+  "update la i v = do {
+      old_v \<leftarrow> lookup la i;
+      new_la \<leftarrow> update_aux la i v;
+      la :=\<^sub>R Upd i old_v new_la;
       return new_la
   }"
 declare update.simps[code]
@@ -227,93 +356,6 @@ declare update.simps[code]
 find_theorems "<_> Array.upd _ _ _ <_>"
 
 find_consts "(_ \<Rightarrow> _ list) \<Rightarrow> _ list \<Rightarrow> _ list"
-
-(* WRONG! Old needs old value!*)
-abbreviation update' where
-  "update' new_p old_p i old_v \<equiv>
-    List.maps (
-      \<lambda>(p, c).
-        if old_p = p 
-        then [(p, Upd' i old_v new_p), (new_p, c)]
-        else [(p, c)]
-      )"
-
-lemma update: "
-   <master_assn t * \<up>(la_rel' t n xs a \<and> i < length xs)> 
-      update a i x
-   <\<lambda>r. let new_t = update' r a i (xs!i) t
-        in master_assn new_t * \<up>(la_rel' new_t n (xs[i := x]) r \<and> la_rel' new_t (Suc n) xs a)
-   >\<^sub>t"
-proof(induction n)
-  case 0
-  then show ?case
-    using lookup[of t 0 xs a i] 
-    apply(sep_auto simp: Let_def update.simps)
-     apply(subst open_master_assn, assumption)
-     apply sep_auto
-    (* Why "<true * true>" ? *)
-    subgoal for xa xaa
-      apply(cases xaa)
-       apply sep_auto
-     
-      sorry
-    sorry
-next
-  case (Suc n)
-  then show ?case 
-     using lookup[of t "Suc n" xs a i]   
-    apply(sep_auto simp: update.simps)
-       apply(subst open_master_assn, assumption)
-     apply sep_auto
-    sorry
-qed
-(*proof(induction n)
-  case 0
-  
-
-  then show ?case
-     using lookup[of t 0 xs a i]   
-    apply(sep_auto simp: update.simps)
-      apply(subst open_master_assn, assumption)
-      apply(sep_auto)
-     sorry
-next
-  case (Suc n)
-  then show ?case
-    using lookup[of t "Suc n" xs a i]   
-    apply(sep_auto simp: update.simps)
-      apply(subst open_master_assn, assumption)
-      apply(sep_auto)
-     apply(subst open_master_assn, assumption)
-    apply sep_auto
-    subgoal for ia xa a' xs' xaa
-      apply sep_auto
-      using close_master_assn_upd'[of a ia xa a' t] 
-        apply sep_auto
-      using Suc.IH
-        apply sep_auto
-     sorry
-    sorry
-    (*subgoal for  ia xa a' xs' 
-    proof(induction xaa)
-      case (Array x)
-      then show ?case by auto
-    next
-      case (Upd x1a x2 x3)
-      then show ?case 
-        using close_master_assn_upd'[of a ia xa a' t]
-        apply sep_auto
-        using close_master_assn_upd'[of a ia xa a' t]
-            apply sep_auto
-        thm Suc
-        using Suc.IH apply sep_auto
-        sorry
-    qed*)
-qed*)
-
-  (*using lookup[of t n xs a i]
-  apply(sep_auto simp: update.simps)
-  apply(subst open_master_assn, assumption)*)
 
  
 definition create_la where
@@ -325,8 +367,9 @@ definition create_la where
 
 definition test where "test = do {
   r \<leftarrow> create_la 3 (5::nat);
-  y \<leftarrow> update r 1 (6::nat);
-  x \<leftarrow> lookup y 2;
+  y \<leftarrow> update r 1 (9::nat);
+  y \<leftarrow> update y 1 (7::nat);
+  x \<leftarrow> lookup y 1;
   return x
 }"
 
